@prefix : <http://eminent.intnet.eu/vocabulary#> .
@prefix owl: <http://www.w3.org/2002/07/owl#> .
@prefix rdf: <http://www.w3.org/1999/02/22-rdf-syntax-ns#> .
@prefix xml: <http://www.w3.org/XML/1998/namespace> .
@prefix xsd: <http://www.w3.org/2001/XMLSchema#> .
@prefix rdfs: <http://www.w3.org/2000/01/rdf-schema#> .
@prefix skos: <http://www.w3.org/2004/02/skos/core#> .
@prefix dcterms: <http://purl.org/dc/terms/> .
@prefix eminent: <http://eminent.intnet.eu/vocabulary#> .
@base <http://eminent.intnet.eu/vocabulary#> .

<http://eminent.intnet.eu/vocabulary#> rdf:type owl:Ontology ;
                                        owl:imports <http://sgam.intnet.eu/vocabulary#> ,
                                                    <http://www.w3.org/2004/02/skos/core> ;
                                        dcterms:creator "AIT" ,
                                                        "EPRI" ,
                                                        "OFFIS" ;
                                        rdfs:comment """This vocabulary was created in the context of the int:net Horizon project to document the  
concepts used in the Eminent Maturity model.""" ;
                                        skos:prefLabel "Eminent Vocabulary"@en .

#################################################################
#    Individuals
#################################################################

###  http://eminent.intnet.eu/vocabulary#
<http://eminent.intnet.eu/vocabulary#> rdf:type owl:NamedIndividual ,
                                                skos:ConceptScheme .


###  http://eminent.intnet.eu/vocabulary#c37aa227_44a2_4c11_8507_e4d28267c7ab
eminent:c37aa227_44a2_4c11_8507_e4d28267c7ab rdf:type owl:NamedIndividual ,
                                                      skos:Concept ;
                                             skos:topConceptOf <http://eminent.intnet.eu/vocabulary#> ;
                                             skos:definition "A group of iorganizations and individuals tha (should) work together to realize interoperability in the context of a certain usecase."@en ;
                                             skos:prefLabel "Community"@en .


###  http://eminent.intnet.eu/vocabulary#c5d4fe14_ee57_4b00_99fb_1e3f98e89c05
eminent:c5d4fe14_ee57_4b00_99fb_1e3f98e89c05 rdf:type owl:NamedIndividual ,
                                                      skos:Concept ;
                                             skos:topConceptOf <http://eminent.intnet.eu/vocabulary#> ;
                                             skos:definition "Testing is the process which is used to identify characteristics or problems of a product, service or system."@en ;
                                             skos:prefLabel "Testing"@en ;
                                             skos:scopeNote "Testing is often carried out by dedicated test facilities that provide the expertise and infrastructure required for performing tests."@en .


###  http://eminent.intnet.eu/vocabulary#d2ba4708_4a59_4225_8dc5_307da0add88a
eminent:d2ba4708_4a59_4225_8dc5_307da0add88a rdf:type owl:NamedIndividual ,
                                                      skos:Concept ;
                                             dcterms:contributor "OFFIS" ;
                                             skos:definition "Interoperability Profiles refer to standardized specifications or sets of protocols that define the specific requirements and capabilities for achieving interoperability between different systems, components, or entities within a given domain."@en ;
                                             skos:prefLabel "Intergration Profiles"@en .


###  http://eminent.intnet.eu/vocabulary#d4e25ae1_5729_4592_af64_68517992e378
eminent:d4e25ae1_5729_4592_af64_68517992e378 rdf:type owl:NamedIndividual ,
                                                      skos:Concept ;
                                             skos:prefLabel "2.3 Compliance Testing"@en .


###  http://eminent.intnet.eu/vocabulary#df690c87_ef6d_4f0e_9f21_83322e3bdc29
eminent:df690c87_ef6d_4f0e_9f21_83322e3bdc29 rdf:type owl:NamedIndividual ,
                                                      skos:Concept ;
                                             skos:prefLabel "Resources"@en .


###  http://eminent.intnet.eu/vocabulary#dfe4dfda_6d42_4274_ab03_29f583468dc9
eminent:dfe4dfda_6d42_4274_ab03_29f583468dc9 rdf:type owl:NamedIndividual ,
                                                      skos:Concept ;
                                             skos:narrower eminent:e68e8760_25e8_45e4_af76_dfdf9cff0f75 ,
                                                           <http://eminent.intnet.eu/vocabulary#1574ed35_24c3_4dc2_b6ba_7a85f7ea5630> ;
                                             skos:topConceptOf <http://eminent.intnet.eu/vocabulary#> ;
                                             skos:definition "A model to compare an organization or communities maturity to in the context of a specific domain"@en ;
                                             skos:prefLabel "Maturity Model"@en ;
                                             skos:scopeNote "In the context of int:net, the maturity is aimed at measuring a communities (or industries) maturity when it comes to interoperability."@en .


###  http://eminent.intnet.eu/vocabulary#e07308d2_a869_45f4_9901_e06c94928eb7
eminent:e07308d2_a869_45f4_9901_e06c94928eb7 rdf:type owl:NamedIndividual ,
                                                      skos:Concept ;
                                             skos:prefLabel "1.2 Knowledge retention"@en .


###  http://eminent.intnet.eu/vocabulary#e5dd5934_7601_43e6_849e_308670327cfc
eminent:e5dd5934_7601_43e6_849e_308670327cfc rdf:type owl:NamedIndividual ,
                                                      skos:Concept ;
                                             skos:prefLabel "3.1 User Base Growth"@en .


###  http://eminent.intnet.eu/vocabulary#e68e8760_25e8_45e4_af76_dfdf9cff0f75
eminent:e68e8760_25e8_45e4_af76_dfdf9cff0f75 rdf:type owl:NamedIndividual ,
                                                      skos:Concept ;
                                             skos:broader eminent:dfe4dfda_6d42_4274_ab03_29f583468dc9 ;
                                             dcterms:contributor "EPRI" ;
                                             skos:definition "A condition that when it's met implies something about the maturity of the subject of study in the related dimension."@en ;
                                             skos:prefLabel "Characteristic"@en .


###  http://eminent.intnet.eu/vocabulary#f67bee8d_4578_42c0_9294_288ed39f9f0b
eminent:f67bee8d_4578_42c0_9294_288ed39f9f0b rdf:type owl:NamedIndividual ,
                                                      skos:Concept ;
                                             skos:prefLabel "People and Organization"@en .


###  http://eminent.intnet.eu/vocabulary#0d86cc07_aa82_4177_8e7a_8726752d17e8
<http://eminent.intnet.eu/vocabulary#0d86cc07_aa82_4177_8e7a_8726752d17e8> rdf:type owl:NamedIndividual ,
                                                                                    skos:Concept ;
                                                                           skos:prefLabel "3.2 Operational Alignment"@en .


###  http://eminent.intnet.eu/vocabulary#1c170adc_e892_4a6b_9954_690279e5e999
<http://eminent.intnet.eu/vocabulary#1c170adc_e892_4a6b_9954_690279e5e999> rdf:type owl:NamedIndividual ,
                                                                                    skos:Concept ;
                                                                           skos:narrower <http://eminent.intnet.eu/vocabulary#51495aa4_9db7_4b68_87af_fd058c1c21b4> ,
                                                                                         <http://eminent.intnet.eu/vocabulary#62e1b06d_9c67_47d7_a757_cfd25f94bb8c> ,
                                                                                         <http://eminent.intnet.eu/vocabulary#63b07d64_e9fb_46de_aa64_eaa118fc6277> ;
                                                                           skos:prefLabel "Capability"@en .


###  http://eminent.intnet.eu/vocabulary#1574ed35_24c3_4dc2_b6ba_7a85f7ea5630
<http://eminent.intnet.eu/vocabulary#1574ed35_24c3_4dc2_b6ba_7a85f7ea5630> rdf:type owl:NamedIndividual ,
                                                                                    skos:Concept ;
                                                                           skos:definition "A question that is aimed at qualifying or quantifying the performance of the subject in a specific dimension by verifying if a certain characteristic is being met."@en ;
                                                                           skos:prefLabel "Question"@en .


###  http://eminent.intnet.eu/vocabulary#2a5b4b54_dd84_4eab_8d53_34a37a7612dd
<http://eminent.intnet.eu/vocabulary#2a5b4b54_dd84_4eab_8d53_34a37a7612dd> rdf:type owl:NamedIndividual ,
                                                                                    skos:Concept ;
                                                                           skos:prefLabel "2.2 Standardization"@en .


###  http://eminent.intnet.eu/vocabulary#2b3896be_7948_49e7_bc73_1748edfaf8f4
<http://eminent.intnet.eu/vocabulary#2b3896be_7948_49e7_bc73_1748edfaf8f4> rdf:type owl:NamedIndividual ,
                                                                                    skos:Concept ;
                                                                           skos:prefLabel "1.3 Diversity Of perspectives"@en .


###  http://eminent.intnet.eu/vocabulary#31e4021e_6b5c_4e7b_b928_b7150b49e788
<http://eminent.intnet.eu/vocabulary#31e4021e_6b5c_4e7b_b928_b7150b49e788> rdf:type owl:NamedIndividual ,
                                                                                    skos:Concept ;
                                                                           skos:prefLabel "1.1 Community Growth"@en .


###  http://eminent.intnet.eu/vocabulary#310de534_15ef_4b12_9bb9_85ce7175c398
<http://eminent.intnet.eu/vocabulary#310de534_15ef_4b12_9bb9_85ce7175c398> rdf:type owl:NamedIndividual ,
                                                                                    skos:Concept ;
                                                                           skos:prefLabel "Information"@en .


###  http://eminent.intnet.eu/vocabulary#4f1fd2ab_7f37_48b2_81cf_7e6582d0d9f2
<http://eminent.intnet.eu/vocabulary#4f1fd2ab_7f37_48b2_81cf_7e6582d0d9f2> rdf:type owl:NamedIndividual ,
                                                                                    skos:Concept ;
                                                                           skos:prefLabel "2.1 Intergation Profile Establishment"@en .


###  http://eminent.intnet.eu/vocabulary#4002a1bb_406e_4c21_8d81_d3e4d41def11
<http://eminent.intnet.eu/vocabulary#4002a1bb_406e_4c21_8d81_d3e4d41def11> rdf:type owl:NamedIndividual ,
                                                                                    skos:Concept ;
                                                                           skos:narrower <http://eminent.intnet.eu/vocabulary#666d4256_e8bf_4615_9a2f_4e9b40d4fdea> ;
                                                                           skos:prefLabel "3.3 Tool, Product, and Reference Implementation Development"@en .


###  http://eminent.intnet.eu/vocabulary#5b64eeef_d3c4_4ee3_91fa_b45d37c09037
<http://eminent.intnet.eu/vocabulary#5b64eeef_d3c4_4ee3_91fa_b45d37c09037> rdf:type owl:NamedIndividual ,
                                                                                    skos:Concept ;
                                                                           dcterms:contributor "OFFIS" ;
                                                                           skos:definition "A use case is a specification of a set of actions performed by a system, which yields an observable result that is, typically, of value for one or more actors or other stakeholders of the system "@en ;
                                                                           skos:prefLabel "Use Cases"@en ;
                                                                           skos:scopeNote "Based on IEC 62559-2:2015 "@en .


###  http://eminent.intnet.eu/vocabulary#5cc05b37_0098_48e0_a633_fc4ac3435634
<http://eminent.intnet.eu/vocabulary#5cc05b37_0098_48e0_a633_fc4ac3435634> rdf:type owl:NamedIndividual ,
                                                                                    skos:Concept ;
                                                                           skos:prefLabel "Process"@en .


###  http://eminent.intnet.eu/vocabulary#51495aa4_9db7_4b68_87af_fd058c1c21b4
<http://eminent.intnet.eu/vocabulary#51495aa4_9db7_4b68_87af_fd058c1c21b4> rdf:type owl:NamedIndividual ,
                                                                                    skos:Concept ;
                                                                           skos:narrower eminent:e07308d2_a869_45f4_9901_e06c94928eb7 ,
                                                                                         <http://eminent.intnet.eu/vocabulary#2b3896be_7948_49e7_bc73_1748edfaf8f4> ,
                                                                                         <http://eminent.intnet.eu/vocabulary#31e4021e_6b5c_4e7b_b928_b7150b49e788> ;
                                                                           skos:prefLabel "1. Community Facilitation"@en .


###  http://eminent.intnet.eu/vocabulary#62e1b06d_9c67_47d7_a757_cfd25f94bb8c
<http://eminent.intnet.eu/vocabulary#62e1b06d_9c67_47d7_a757_cfd25f94bb8c> rdf:type owl:NamedIndividual ,
                                                                                    skos:Concept ;
                                                                           skos:narrower eminent:e5dd5934_7601_43e6_849e_308670327cfc ,
                                                                                         <http://eminent.intnet.eu/vocabulary#0d86cc07_aa82_4177_8e7a_8726752d17e8> ,
                                                                                         <http://eminent.intnet.eu/vocabulary#4002a1bb_406e_4c21_8d81_d3e4d41def11> ,
                                                                                         <http://eminent.intnet.eu/vocabulary#666d4256_e8bf_4615_9a2f_4e9b40d4fdea> ;
                                                                           skos:prefLabel "3. Facilitating Adoption"@en .


###  http://eminent.intnet.eu/vocabulary#63b07d64_e9fb_46de_aa64_eaa118fc6277
<http://eminent.intnet.eu/vocabulary#63b07d64_e9fb_46de_aa64_eaa118fc6277> rdf:type owl:NamedIndividual ,
                                                                                    skos:Concept ;
                                                                           skos:narrower eminent:d4e25ae1_5729_4592_af64_68517992e378 ,
                                                                                         <http://eminent.intnet.eu/vocabulary#2a5b4b54_dd84_4eab_8d53_34a37a7612dd> ,
                                                                                         <http://eminent.intnet.eu/vocabulary#4f1fd2ab_7f37_48b2_81cf_7e6582d0d9f2> ;
                                                                           skos:prefLabel "2. Making Technical Agreements"@en .


###  http://eminent.intnet.eu/vocabulary#6561e6d3_7af9_4f6a_88e9_bfae1125a547
<http://eminent.intnet.eu/vocabulary#6561e6d3_7af9_4f6a_88e9_bfae1125a547> rdf:type owl:NamedIndividual ,
                                                                                    skos:Concept ;
                                                                           skos:related eminent:dfe4dfda_6d42_4274_ab03_29f583468dc9 ;
                                                                           skos:topConceptOf <http://eminent.intnet.eu/vocabulary#> ;
                                                                           dcterms:contributor "EPRI" ;
                                                                           skos:definition "The excersize of comparing an organizations or communities maturity to a maturity model to determine overal performance comapared to peers and identify areas of improvement."@en ;
                                                                           skos:prefLabel "Maturity Assessment"@en .


###  http://eminent.intnet.eu/vocabulary#666d4256_e8bf_4615_9a2f_4e9b40d4fdea
<http://eminent.intnet.eu/vocabulary#666d4256_e8bf_4615_9a2f_4e9b40d4fdea> rdf:type owl:NamedIndividual ,
                                                                                    skos:Concept ;
                                                                           skos:prefLabel "3.4 Market Creation"@en .


###  http://eminent.intnet.eu/vocabulary#8f586df0_67bb_4e22_b6e3_18bd9c0fae7b
<http://eminent.intnet.eu/vocabulary#8f586df0_67bb_4e22_b6e3_18bd9c0fae7b> rdf:type owl:NamedIndividual ,
                                                                                    skos:Concept ;
                                                                           skos:related eminent:c5d4fe14_ee57_4b00_99fb_1e3f98e89c05 ;
                                                                           dcterms:contributor "AIT" ;
                                                                           skos:definition "Compliance means that a product or service conforms with the requirements of a specification, technical standard, or regulation."@en ;
                                                                           skos:prefLabel "Compliance"@en .


###  http://eminent.intnet.eu/vocabulary#8fa61830_69c7_4bf4_940e_cd7c4a21e195
<http://eminent.intnet.eu/vocabulary#8fa61830_69c7_4bf4_940e_cd7c4a21e195> rdf:type owl:NamedIndividual ,
                                                                                    skos:Concept ;
                                                                           skos:narrower eminent:df690c87_ef6d_4f0e_9f21_83322e3bdc29 ,
                                                                                         eminent:f67bee8d_4578_42c0_9294_288ed39f9f0b ,
                                                                                         <http://eminent.intnet.eu/vocabulary#310de534_15ef_4b12_9bb9_85ce7175c398> ,
                                                                                         <http://eminent.intnet.eu/vocabulary#5cc05b37_0098_48e0_a633_fc4ac3435634> ;
                                                                           skos:prefLabel "Dimension"@en .


###  Generated by the OWL API (version 4.5.26.2023-07-17T20:34:13Z) https://github.com/owlcs/owlapi
