@prefix : <http://eminent.intnet.eu/ontology#> .
@prefix owl: <http://www.w3.org/2002/07/owl#> .
@prefix rdf: <http://www.w3.org/1999/02/22-rdf-syntax-ns#> .
@prefix xml: <http://www.w3.org/XML/1998/namespace> .
@prefix xsd: <http://www.w3.org/2001/XMLSchema#> .
@prefix rdfs: <http://www.w3.org/2000/01/rdf-schema#> .
@prefix intnet: <http://eminent.intnet.eu/ontology#/> .
@base <http://eminent.intnet.eu/ontology#> .

<http://eminent.intnet.eu/ontology#> rdf:type owl:Ontology ;
                                      owl:imports <http://eminent.intnet.eu/vocabulary#> ,
                                                  <http://purl.org/dc/terms/> ,
                                                  <http://www.w3.org/ns/sosa/> .

#################################################################
#    Object Properties
#################################################################

###  http://eminent.intnet.eu/ontology#measures
:measures rdf:type owl:ObjectProperty ;
          rdfs:domain <http://www.w3.org/ns/sosa/Procedure> ;
          rdfs:range <http://www.w3.org/ns/sosa/ObservableProperty> ;
          rdfs:comment "the relation between a procedure and what it is intended to measure."@en .


#################################################################
#    Data properties
#################################################################

###  http://eminent.intnet.eu/ontology#phrasing
:phrasing rdf:type owl:DatatypeProperty ;
          rdfs:domain :QuestionVersion ;
          rdfs:range rdf:langString .


#################################################################
#    Classes
#################################################################

###  http://eminent.intnet.eu/ontology#Answer
:Answer rdf:type owl:Class ;
        rdfs:subClassOf <http://www.w3.org/ns/sosa/Observation> ;
        <http://www.w3.org/2004/02/skos/core#definition> "A single anwer to a single question. Multiple Answers can be part of an AnswerSet" .


###  http://eminent.intnet.eu/ontology#AnswerSet
:AnswerSet rdf:type owl:Class ;
           rdfs:subClassOf <http://www.w3.org/ns/sosa/Observation> ;
           <http://www.w3.org/2004/02/skos/core#definition> "A collection of answers to a questionnaire or interview."@en .


###  http://eminent.intnet.eu/ontology#Capability
:Capability rdf:type owl:Class ;
            rdfs:subClassOf <http://www.w3.org/ns/sosa/ObservableProperty> ;
            <http://www.w3.org/2004/02/skos/core#definition> "A capability is a (organizational) skill or ability that an organization needs to have in order to be able to realize its goals or purposes" .


###  http://eminent.intnet.eu/ontology#Characteristic
:Characteristic rdf:type owl:Class ;
                rdfs:subClassOf <http://www.w3.org/ns/sosa/ObservableProperty> ;
                <http://www.w3.org/2004/02/skos/core#definition> "A characteristic is a descrioption of observable qualities that describe a particular maturity lavel fort a specific dimension of a specific capability."@en .


###  http://eminent.intnet.eu/ontology#Dimension
:Dimension rdf:type owl:Class ;
           rdfs:subClassOf <http://www.w3.org/ns/sosa/ObservableProperty> ;
           <http://www.w3.org/2004/02/skos/core#definition> "A dimension, as part of a maturity model, is a recurring perspective through which all capabilities are viewed. Maturity level characteristics are expressed per dimension."@en .


###  http://eminent.intnet.eu/ontology#Question
:Question rdf:type owl:Class ;
          rdfs:subClassOf <http://www.w3.org/ns/sosa/Procedure> ;
          <http://www.w3.org/2004/02/skos/core#definition> "An Individual question, may be part of a questionaire" .


###  http://eminent.intnet.eu/ontology#QuestionVersion
:QuestionVersion rdf:type owl:Class ;
                 rdfs:subClassOf :Question ;
                 <http://www.w3.org/2004/02/skos/core#definition> "A specific version of a question. Typically with an updated phrasing." .


###  http://eminent.intnet.eu/ontology#Questionnaire
:Questionnaire rdf:type owl:Class ;
               rdfs:subClassOf <http://www.w3.org/ns/sosa/Procedure> ;
               <http://www.w3.org/2004/02/skos/core#definition> "A list of questions grouped for the purpose of a study." .


###  http://eminent.intnet.eu/ontology#QuestionnaireVersion
:QuestionnaireVersion rdf:type owl:Class ;
                      rdfs:subClassOf :Questionnaire ;
                      <http://www.w3.org/2004/02/skos/core#definition> "A specific version of a questionnaire" .


###  Generated by the OWL API (version 4.5.26.2023-07-17T20:34:13Z) https://github.com/owlcs/owlapi
