@prefix : <http://eminent.intnet.eu/vocabulary#> .
@prefix owl: <http://www.w3.org/2002/07/owl#> .
@prefix rdf: <http://www.w3.org/1999/02/22-rdf-syntax-ns#> .
@prefix xml: <http://www.w3.org/XML/1998/namespace> .
@prefix xsd: <http://www.w3.org/2001/XMLSchema#> .
@prefix rdfs: <http://www.w3.org/2000/01/rdf-schema#> .
@prefix skos: <http://www.w3.org/2004/02/skos/core#> .
@prefix dcterms: <http://purl.org/dc/terms/> .
@prefix eminent: <http://eminent.intnet.eu/vocabulary#> .
@base <http://eminent.intnet.eu/vocabulary#> .

<http://eminent.intnet.eu/vocabulary#> rdf:type owl:Ontology ;
                                        owl:imports <http://www.w3.org/2004/02/skos/core> ;
                                        dcterms:creator "AIT" ,
                                                        "EPRI" ,
                                                        "OFFIS" ;
                                        rdfs:comment """This vocabulary was created in the context of the int:net Horizon project to document the  
concepts used in the Eminent Maturity model.""" ;
                                        skos:prefLabel "Eminent Vocabulary" .

#################################################################
#    Datatypes
#################################################################

###  http://purl.org/dc/terms/Box
dcterms:Box rdf:type rdfs:Datatype .


###  http://purl.org/dc/terms/ISO3166
dcterms:ISO3166 rdf:type rdfs:Datatype .


###  http://purl.org/dc/terms/ISO639-2
dcterms:ISO639-2 rdf:type rdfs:Datatype .


###  http://purl.org/dc/terms/ISO639-3
dcterms:ISO639-3 rdf:type rdfs:Datatype .


###  http://purl.org/dc/terms/Period
dcterms:Period rdf:type rdfs:Datatype .


###  http://purl.org/dc/terms/Point
dcterms:Point rdf:type rdfs:Datatype .


###  http://purl.org/dc/terms/RFC1766
dcterms:RFC1766 rdf:type rdfs:Datatype .


###  http://purl.org/dc/terms/RFC3066
dcterms:RFC3066 rdf:type rdfs:Datatype .


###  http://purl.org/dc/terms/RFC4646
dcterms:RFC4646 rdf:type rdfs:Datatype .


###  http://purl.org/dc/terms/RFC5646
dcterms:RFC5646 rdf:type rdfs:Datatype .


###  http://purl.org/dc/terms/URI
dcterms:URI rdf:type rdfs:Datatype .


###  http://purl.org/dc/terms/W3CDTF
dcterms:W3CDTF rdf:type rdfs:Datatype .


#################################################################
#    Classes
#################################################################

###  http://purl.org/dc/terms/Agent
dcterms:Agent rdf:type owl:Class .


###  http://purl.org/dc/terms/AgentClass
dcterms:AgentClass rdf:type owl:Class .


###  http://purl.org/dc/terms/BibliographicResource
dcterms:BibliographicResource rdf:type owl:Class .


###  http://purl.org/dc/terms/FileFormat
dcterms:FileFormat rdf:type owl:Class .


###  http://purl.org/dc/terms/Frequency
dcterms:Frequency rdf:type owl:Class .


###  http://purl.org/dc/terms/Jurisdiction
dcterms:Jurisdiction rdf:type owl:Class .


###  http://purl.org/dc/terms/LicenseDocument
dcterms:LicenseDocument rdf:type owl:Class .


###  http://purl.org/dc/terms/LinguisticSystem
dcterms:LinguisticSystem rdf:type owl:Class .


###  http://purl.org/dc/terms/Location
dcterms:Location rdf:type owl:Class .


###  http://purl.org/dc/terms/LocationPeriodOrJurisdiction
dcterms:LocationPeriodOrJurisdiction rdf:type owl:Class .


###  http://purl.org/dc/terms/MediaType
dcterms:MediaType rdf:type owl:Class .


###  http://purl.org/dc/terms/MediaTypeOrExtent
dcterms:MediaTypeOrExtent rdf:type owl:Class .


###  http://purl.org/dc/terms/MethodOfAccrual
dcterms:MethodOfAccrual rdf:type owl:Class .


###  http://purl.org/dc/terms/MethodOfInstruction
dcterms:MethodOfInstruction rdf:type owl:Class .


###  http://purl.org/dc/terms/PeriodOfTime
dcterms:PeriodOfTime rdf:type owl:Class .


###  http://purl.org/dc/terms/PhysicalMedium
dcterms:PhysicalMedium rdf:type owl:Class .


###  http://purl.org/dc/terms/PhysicalResource
dcterms:PhysicalResource rdf:type owl:Class .


###  http://purl.org/dc/terms/Policy
dcterms:Policy rdf:type owl:Class .


###  http://purl.org/dc/terms/ProvenanceStatement
dcterms:ProvenanceStatement rdf:type owl:Class .


###  http://purl.org/dc/terms/RightsStatement
dcterms:RightsStatement rdf:type owl:Class .


###  http://purl.org/dc/terms/SizeOrDuration
dcterms:SizeOrDuration rdf:type owl:Class .


###  http://purl.org/dc/terms/Standard
dcterms:Standard rdf:type owl:Class .


#################################################################
#    Individuals
#################################################################

###  http://eminent.intnet.eu/vocabulary#
<http://eminent.intnet.eu/vocabulary#> rdf:type owl:NamedIndividual ,
                                                skos:ConceptScheme .


###  http://eminent.intnet.eu/vocabulary#a02ca9a4_7c5e_4ae7_aaba_2798950f3762
eminent:a02ca9a4_7c5e_4ae7_aaba_2798950f3762 rdf:type owl:NamedIndividual ,
                                                      skos:Concept ;
                                             skos:related <http://eminent.intnet.eu/vocabulary#8eadbfea_138f_4007_b87e_da970d65b7f9> ;
                                             dcterms:contributor "OFFIS" ;
                                             skos:definition "The function layer describes system use cases, functions and services including their relationships from an architectural viewpoint. "@en ;
                                             skos:prefLabel "Function Layer"@en ;
                                             skos:scopeNote "According to the SGAM User Manual (https://www.cencenelec.eu/media/CEN-CENELEC/AreasOfWork/CEN-CENELEC_Topics/Smart%20Grids%20and%20Meters/Smart%20Grids/4_sgcg_methodology_sgamusermanual.pdf)"@en .


###  http://eminent.intnet.eu/vocabulary#b2a3426f_7139_4db2_b9f5_b4b3cb2d3c8d
eminent:b2a3426f_7139_4db2_b9f5_b4b3cb2d3c8d rdf:type owl:NamedIndividual ,
                                                      skos:Concept ;
                                             skos:related <http://eminent.intnet.eu/vocabulary#79a8c9db_8a04_4c68_87f8_c007becbc4fe> ;
                                             dcterms:contributor "EPRI" ;
                                             skos:definition "Data integrity refers to the requirement that data when represemnts the same and has the same intent as when it was recorded."@en ;
                                             skos:prefLabel "Data Intergrity"@en ;
                                             skos:scopeNote "Changes in formator corrections for data quality purposes do not constitute a loss of integrity because while the data has been changed the intent is the same"@en .


###  http://eminent.intnet.eu/vocabulary#b4fe6283_38d3_44e5_afb5_7572c386efaa
eminent:b4fe6283_38d3_44e5_afb5_7572c386efaa rdf:type owl:NamedIndividual ,
                                                      skos:Concept ;
                                             skos:prefLabel "Data Quality"@en .


###  http://eminent.intnet.eu/vocabulary#b99b7b63_dddb_47e5_a215_3034d4d75d41
eminent:b99b7b63_dddb_47e5_a215_3034d4d75d41 rdf:type owl:NamedIndividual ,
                                                      skos:Concept ;
                                             skos:broader eminent:dfe4dfda_6d42_4274_ab03_29f583468dc9 ,
                                                          <http://eminent.intnet.eu/vocabulary#9bcd5305_1500_43c6_bdff_3d8c21c4f101> ;
                                             dcterms:contributor "EPRI" ;
                                             skos:definition "Typically a capability or aspect of maturity in a specific category."@en ;
                                             skos:prefLabel "Dimension"@en .


###  http://eminent.intnet.eu/vocabulary#c37aa227_44a2_4c11_8507_e4d28267c7ab
eminent:c37aa227_44a2_4c11_8507_e4d28267c7ab rdf:type owl:NamedIndividual ,
                                                      skos:Concept ;
                                             skos:topConceptOf <http://eminent.intnet.eu/vocabulary#> ;
                                             skos:definition "A group of iorganizations and individuals tha (should) work together to realize interoperability in the context of a certain usecase."@en ;
                                             skos:prefLabel "Community"@en .


###  http://eminent.intnet.eu/vocabulary#c5d4fe14_ee57_4b00_99fb_1e3f98e89c05
eminent:c5d4fe14_ee57_4b00_99fb_1e3f98e89c05 rdf:type owl:NamedIndividual ,
                                                      skos:Concept ;
                                             skos:topConceptOf <http://eminent.intnet.eu/vocabulary#> ;
                                             skos:definition "Testing is the process which is used to identify characteristics or problems of a product, service or system."@en ;
                                             skos:prefLabel "Testing"@en ;
                                             skos:scopeNote "Testing is often carried out by dedicated test facilities that provide the expertise and infrastructure required for performing tests."@en .


###  http://eminent.intnet.eu/vocabulary#d2ba4708_4a59_4225_8dc5_307da0add88a
eminent:d2ba4708_4a59_4225_8dc5_307da0add88a rdf:type owl:NamedIndividual ,
                                                      skos:Concept ;
                                             skos:broader eminent:e550a9ec_f846_44af_92e1_f0f86131f448 ;
                                             dcterms:contributor "OFFIS" ;
                                             skos:definition "Interoperability Profiles refer to standardized specifications or sets of protocols that define the specific requirements and capabilities for achieving interoperability between different systems, components, or entities within a given domain."@en ;
                                             skos:prefLabel "Intergration Profiles"@en .


###  http://eminent.intnet.eu/vocabulary#d95356d2_49eb_4436_a7c5_fae01b48f8d2
eminent:d95356d2_49eb_4436_a7c5_fae01b48f8d2 rdf:type owl:NamedIndividual ,
                                                      skos:Concept ;
                                             skos:definition "The regulation layer represents the regulatory view of a community on a regional, national, association of nations or international basis."@en ;
                                             skos:prefLabel "Regulation Layer"@en ;
                                             skos:scopeNote "According to the work of T2.1 (needs to be updated with a consensus of T2.2)"@en .


###  http://eminent.intnet.eu/vocabulary#dfe4dfda_6d42_4274_ab03_29f583468dc9
eminent:dfe4dfda_6d42_4274_ab03_29f583468dc9 rdf:type owl:NamedIndividual ,
                                                      skos:Concept ;
                                             skos:narrower eminent:b99b7b63_dddb_47e5_a215_3034d4d75d41 ,
                                                           eminent:e68e8760_25e8_45e4_af76_dfdf9cff0f75 ,
                                                           <http://eminent.intnet.eu/vocabulary#1574ed35_24c3_4dc2_b6ba_7a85f7ea5630> ,
                                                           <http://eminent.intnet.eu/vocabulary#9bcd5305_1500_43c6_bdff_3d8c21c4f101> ;
                                             skos:topConceptOf <http://eminent.intnet.eu/vocabulary#> ;
                                             skos:definition "A model to compare an organization or communities maturity to in the context of a specific domain"@en ;
                                             skos:prefLabel "Maturity Model"@en ;
                                             skos:scopeNote "In the context of int:net, the maturity is aimed at measuring a communities (or industries) maturity when it comes to interoperability."@en .


###  http://eminent.intnet.eu/vocabulary#e550a9ec_f846_44af_92e1_f0f86131f448
eminent:e550a9ec_f846_44af_92e1_f0f86131f448 rdf:type owl:NamedIndividual ,
                                                      skos:Concept ;
                                             skos:narrower eminent:d2ba4708_4a59_4225_8dc5_307da0add88a ,
                                                           <http://eminent.intnet.eu/vocabulary#23153956_61c8_4748_acef_4a1e192a45b4> ;
                                             skos:topConceptOf <http://eminent.intnet.eu/vocabulary#> ;
                                             dcterms:contributor "OFFIS" ;
                                             skos:definition "Documentation represents an essential point to ensure a common understanding of the community"@en ;
                                             skos:prefLabel "Documentation"@en ;
                                             skos:scopeNote "Based on D2.1"@en .


###  http://eminent.intnet.eu/vocabulary#e59f1dac_3d34_45b4_b3f2_45c0f91185c7
eminent:e59f1dac_3d34_45b4_b3f2_45c0f91185c7 rdf:type owl:NamedIndividual ,
                                                      skos:Concept ;
                                             skos:broader <http://eminent.intnet.eu/vocabulary#8eadbfea_138f_4007_b87e_da970d65b7f9> ;
                                             dcterms:contributor "OFFIS" ;
                                             skos:definition "The business layer represents the business view on the information exchange related to smart grids."@en ;
                                             skos:prefLabel "Business Layer"@en ;
                                             skos:scopeNote "According to the SGAM User Manual (https://www.cencenelec.eu/media/CEN-CENELEC/AreasOfWork/CEN-CENELEC_Topics/Smart%20Grids%20and%20Meters/Smart%20Grids/4_sgcg_methodology_sgamusermanual.pdf)"@en .


###  http://eminent.intnet.eu/vocabulary#e68e8760_25e8_45e4_af76_dfdf9cff0f75
eminent:e68e8760_25e8_45e4_af76_dfdf9cff0f75 rdf:type owl:NamedIndividual ,
                                                      skos:Concept ;
                                             skos:broader eminent:b99b7b63_dddb_47e5_a215_3034d4d75d41 ,
                                                          eminent:dfe4dfda_6d42_4274_ab03_29f583468dc9 ;
                                             dcterms:contributor "EPRI" ;
                                             skos:definition "A condition that when it's met implies something about the maturity of the subject of study in the related dimension."@en ;
                                             skos:prefLabel "Characteristic"@en .


###  http://eminent.intnet.eu/vocabulary#ee9e324f_9439_453f_a3da_326e43f4d8a3
eminent:ee9e324f_9439_453f_a3da_326e43f4d8a3 rdf:type owl:NamedIndividual ,
                                                      skos:Concept ;
                                             skos:broader <http://eminent.intnet.eu/vocabulary#6b8a3625_1fa9_4396_a757_7e896b3acf9e> ;
                                             dcterms:contributor "EPRI" ;
                                             skos:definition "Data Sovereignty is about the degree to which data is being used in accordance to the policicies, requrements and restrictions imposed by the owners of the data. "@en ;
                                             skos:prefLabel "Data Sovereignty"@en .


###  http://eminent.intnet.eu/vocabulary#1dd1930a_870a_4d0a_a89c_d634eb63eb8e
<http://eminent.intnet.eu/vocabulary#1dd1930a_870a_4d0a_a89c_d634eb63eb8e> rdf:type owl:NamedIndividual ,
                                                                                    skos:Concept ;
                                                                           skos:related <http://eminent.intnet.eu/vocabulary#79a8c9db_8a04_4c68_87f8_c007becbc4fe> ;
                                                                           dcterms:contributor "EPRI" ;
                                                                           skos:definition "Data availability refers to the degree to which data is accessable to those who need it, when they need it."@en ;
                                                                           skos:prefLabel "Data Availability"@en ;
                                                                           skos:scopeNote "Data availabiltity is mostly influenced by system uptime and redundancy"@en .


###  http://eminent.intnet.eu/vocabulary#1574ed35_24c3_4dc2_b6ba_7a85f7ea5630
<http://eminent.intnet.eu/vocabulary#1574ed35_24c3_4dc2_b6ba_7a85f7ea5630> rdf:type owl:NamedIndividual ,
                                                                                    skos:Concept ;
                                                                           skos:definition "A question that is aimed at qualifying or quantifying the performance of the subject in a specific dimension by verifying if a certain characteristic is being met."@en ;
                                                                           skos:prefLabel "Question"@en .


###  http://eminent.intnet.eu/vocabulary#23153956_61c8_4748_acef_4a1e192a45b4
<http://eminent.intnet.eu/vocabulary#23153956_61c8_4748_acef_4a1e192a45b4> rdf:type owl:NamedIndividual ,
                                                                                    skos:Concept ;
                                                                           skos:broader eminent:e550a9ec_f846_44af_92e1_f0f86131f448 ;
                                                                           skos:narrower <http://eminent.intnet.eu/vocabulary#23153956_61c8_4748_acef_4a1e192a45b4> ,
                                                                                         <http://eminent.intnet.eu/vocabulary#5b64eeef_d3c4_4ee3_91fa_b45d37c09037> ;
                                                                           dcterms:contributor "OFFIS" ;
                                                                           skos:definition "Architecture, refers to the conceptual framework that defines the structure, components, and relationships of a system or domain, enabling the integration and interaction of various elements to achieve desired outcomes."@en ;
                                                                           skos:prefLabel "Architecture"@en .


###  http://eminent.intnet.eu/vocabulary#4a2da955_112a_4ff3_8bb3_5c02005f8e08
<http://eminent.intnet.eu/vocabulary#4a2da955_112a_4ff3_8bb3_5c02005f8e08> rdf:type owl:NamedIndividual ,
                                                                                    skos:Concept ;
                                                                           skos:broader <http://eminent.intnet.eu/vocabulary#8eadbfea_138f_4007_b87e_da970d65b7f9> ;
                                                                           dcterms:contributor "EPRI" ;
                                                                           skos:definition "The information layer describes the information that is being used and exchanged between functions, services and components."@en ;
                                                                           skos:prefLabel "Information Layer"@en ;
                                                                           skos:scopeNote "According to the SGAM User Manual (https://www.cencenelec.eu/media/CEN-CENELEC/AreasOfWork/CEN-CENELEC_Topics/Smart%20Grids%20and%20Meters/Smart%20Grids/4_sgcg_methodology_sgamusermanual.pdf)"@en .


###  http://eminent.intnet.eu/vocabulary#448fb926_b209_415b_a376_38000fd6dc91
<http://eminent.intnet.eu/vocabulary#448fb926_b209_415b_a376_38000fd6dc91> rdf:type owl:NamedIndividual ,
                                                                                    skos:Concept ;
                                                                           skos:related <http://eminent.intnet.eu/vocabulary#6b8a3625_1fa9_4396_a757_7e896b3acf9e> ;
                                                                           skos:altLabel "Business Ownership"@en ;
                                                                           skos:definition "Data role models address how business ownership and other mandates around managing data are assigned."@en ;
                                                                           skos:prefLabel "Data Roles"@en ;
                                                                           skos:scopeNote "Refined rolemodels unsure that \"IT\" isn't just the default manager of data, but that in fact domain experts in the primary business have the mandate and responsibility to manage and maintain their data."@en .


###  http://eminent.intnet.eu/vocabulary#5b64eeef_d3c4_4ee3_91fa_b45d37c09037
<http://eminent.intnet.eu/vocabulary#5b64eeef_d3c4_4ee3_91fa_b45d37c09037> rdf:type owl:NamedIndividual ,
                                                                                    skos:Concept ;
                                                                           skos:broader eminent:e550a9ec_f846_44af_92e1_f0f86131f448 ;
                                                                           dcterms:contributor "OFFIS" ;
                                                                           skos:definition "A use case is a specification of a set of actions performed by a system, which yields an observable result that is, typically, of value for one or more actors or other stakeholders of the system "@en ;
                                                                           skos:prefLabel "Use Cases"@en ;
                                                                           skos:scopeNote "Based on IEC 62559-2:2015 "@en .


###  http://eminent.intnet.eu/vocabulary#6b8a3625_1fa9_4396_a757_7e896b3acf9e
<http://eminent.intnet.eu/vocabulary#6b8a3625_1fa9_4396_a757_7e896b3acf9e> rdf:type owl:NamedIndividual ,
                                                                                    skos:Concept ;
                                                                           skos:topConceptOf <http://eminent.intnet.eu/vocabulary#> ;
                                                                           dcterms:contributor "EPRI" ;
                                                                           skos:definition "The term ‘data space’ refers to a type of data relationship between trusted partners who adhere to the same high level standards and guidelines in relation to data storage and sharing within one or many Vertical Ecosystems."@en ;
                                                                           skos:prefLabel "Data Space"@en ;
                                                                           skos:scopeNote "A critical aspect of the data space notion is that data are not stored centrally, but rather at the source. Thus, they are only transferred through semantic interoperability as necessary. Data in the Gaia-X Data Spaces context are kept exclusively by the Association’s members."@en .


###  http://eminent.intnet.eu/vocabulary#6058bd39_f949_4e8c_9923_b2db3401d6e9
<http://eminent.intnet.eu/vocabulary#6058bd39_f949_4e8c_9923_b2db3401d6e9> rdf:type owl:NamedIndividual ,
                                                                                    skos:Concept ;
                                                                           skos:prefLabel "Reference Data"@en .


###  http://eminent.intnet.eu/vocabulary#6561e6d3_7af9_4f6a_88e9_bfae1125a547
<http://eminent.intnet.eu/vocabulary#6561e6d3_7af9_4f6a_88e9_bfae1125a547> rdf:type owl:NamedIndividual ,
                                                                                    skos:Concept ;
                                                                           skos:related eminent:dfe4dfda_6d42_4274_ab03_29f583468dc9 ;
                                                                           skos:topConceptOf <http://eminent.intnet.eu/vocabulary#> ;
                                                                           dcterms:contributor "EPRI" ;
                                                                           skos:definition "The excersize of comparing an organizations or communities maturity to a maturity model to determine overal performance comapared to peers and identify areas of improvement."@en ;
                                                                           skos:prefLabel "Maturity Assessment"@en .


###  http://eminent.intnet.eu/vocabulary#72bcdea6_418e_4e59_add9_79dcd484cf23
<http://eminent.intnet.eu/vocabulary#72bcdea6_418e_4e59_add9_79dcd484cf23> rdf:type owl:NamedIndividual ,
                                                                                    skos:Concept ;
                                                                           skos:prefLabel "Data Management"@en .


###  http://eminent.intnet.eu/vocabulary#79a8c9db_8a04_4c68_87f8_c007becbc4fe
<http://eminent.intnet.eu/vocabulary#79a8c9db_8a04_4c68_87f8_c007becbc4fe> rdf:type owl:NamedIndividual ,
                                                                                    skos:Concept ;
                                                                           skos:narrower eminent:b2a3426f_7139_4db2_b9f5_b4b3cb2d3c8d ,
                                                                                         <http://eminent.intnet.eu/vocabulary#1dd1930a_870a_4d0a_a89c_d634eb63eb8e> ;
                                                                           skos:topConceptOf <http://eminent.intnet.eu/vocabulary#> ;
                                                                           skos:prefLabel "Information Security"@en .


###  http://eminent.intnet.eu/vocabulary#8eadbfea_138f_4007_b87e_da970d65b7f9
<http://eminent.intnet.eu/vocabulary#8eadbfea_138f_4007_b87e_da970d65b7f9> rdf:type owl:NamedIndividual ,
                                                                                    skos:Concept ;
                                                                           skos:narrower eminent:a02ca9a4_7c5e_4ae7_aaba_2798950f3762 ,
                                                                                         eminent:d95356d2_49eb_4436_a7c5_fae01b48f8d2 ,
                                                                                         eminent:e59f1dac_3d34_45b4_b3f2_45c0f91185c7 ,
                                                                                         <http://eminent.intnet.eu/vocabulary#4a2da955_112a_4ff3_8bb3_5c02005f8e08> ,
                                                                                         <http://eminent.intnet.eu/vocabulary#996258f0_4252_4478_8610_762aafa4c8a6> ;
                                                                           skos:topConceptOf <http://eminent.intnet.eu/vocabulary#> ;
                                                                           dcterms:contributor "OFFIS" ;
                                                                           skos:definition "An interoperability layer refers to a distinct level or component within a system architecture that facilitates the seamless exchange of information and functionality between different interconnected systems or components."@en ;
                                                                           skos:prefLabel "Interoperability Layer"@en .


###  http://eminent.intnet.eu/vocabulary#8f586df0_67bb_4e22_b6e3_18bd9c0fae7b
<http://eminent.intnet.eu/vocabulary#8f586df0_67bb_4e22_b6e3_18bd9c0fae7b> rdf:type owl:NamedIndividual ,
                                                                                    skos:Concept ;
                                                                           skos:related eminent:c5d4fe14_ee57_4b00_99fb_1e3f98e89c05 ;
                                                                           dcterms:contributor "AIT" ;
                                                                           skos:definition "Compliance means that a product or service conforms with the requirements of a specification, technical standard, or regulation."@en ;
                                                                           skos:prefLabel "Compliance"@en .


###  http://eminent.intnet.eu/vocabulary#9bcd5305_1500_43c6_bdff_3d8c21c4f101
<http://eminent.intnet.eu/vocabulary#9bcd5305_1500_43c6_bdff_3d8c21c4f101> rdf:type owl:NamedIndividual ,
                                                                                    skos:Concept ;
                                                                           skos:broader eminent:dfe4dfda_6d42_4274_ab03_29f583468dc9 ;
                                                                           dcterms:contributor "EPRI" ;
                                                                           skos:definition "A grouping of dimensions that together describe a broader aspect of (organizational) maturity."@en ;
                                                                           skos:prefLabel "Category"@en .


###  http://eminent.intnet.eu/vocabulary#95fc579c_c9d3_4ca5_bdf3_394bd2c3a37d
<http://eminent.intnet.eu/vocabulary#95fc579c_c9d3_4ca5_bdf3_394bd2c3a37d> rdf:type owl:NamedIndividual ,
                                                                                    skos:Concept ;
                                                                           skos:broader <http://eminent.intnet.eu/vocabulary#6b8a3625_1fa9_4396_a757_7e896b3acf9e> ;
                                                                           dcterms:contributor "EPRI" ;
                                                                           skos:definition "Data policies are practices and agreements about how data is managed. "@en ;
                                                                           skos:prefLabel "Data Policy Enforcement"@en ;
                                                                           skos:scopeNote "A data space is the sum of all its participants, which may be data providers, users and intermediaries. Data spaces can be nested and overlapping. For instance, a data provider can participate in several data spaces all at once."@en .


###  http://eminent.intnet.eu/vocabulary#996258f0_4252_4478_8610_762aafa4c8a6
<http://eminent.intnet.eu/vocabulary#996258f0_4252_4478_8610_762aafa4c8a6> rdf:type owl:NamedIndividual ,
                                                                                    skos:Concept ;
                                                                           skos:related <http://eminent.intnet.eu/vocabulary#8eadbfea_138f_4007_b87e_da970d65b7f9> ;
                                                                           dcterms:contributor "OFFIS" ;
                                                                           skos:definition "The emphasis of the communication layer is to describe protocols and mechanisms for the interoperable exchange of information between components in the context of the underlying use case, function or service and related information objects or data models."@en ;
                                                                           skos:prefLabel "Communication Layer"@en ;
                                                                           skos:scopeNote "According to the SGAM User Manual (https://www.cencenelec.eu/media/CEN-CENELEC/AreasOfWork/CEN-CENELEC_Topics/Smart%20Grids%20and%20Meters/Smart%20Grids/4_sgcg_methodology_sgamusermanual.pdf)"@en .


###  Generated by the OWL API (version 4.5.25.2023-02-15T19:15:49Z) https://github.com/owlcs/owlapi
